add function example

refinedVST/typing/automation_test.c
@@ -1,0 +1,16 @@
+int main() {
+}
+
+int f_ret_expr() {
+    return 1 + 2;
+}
+
+int f_temps() {
+    int a = 1;
+    int b = 41;
+    return a + b;
+}
+
+int f_call () {
+    return f_temps();
+}
